Here we record some general notes on PDE.

\subsection{Estimates}

Estimates can be used for showing existence of solutions (see the use of Schauder Estimates and the Continuity Method to prove the existence of solutions to elliptic pde), and they may also be used to show control over how our solutions depend on the coefficients in our equations.

\begin{example}
Consider the boundary value problem
\begin{equation}
\begin{cases}
y'' - y = f_\epsilon(x) & 0<x<1,\\
y(0) = 0,\\
y(1) = 0,
\end{cases}
\end{equation}
where $f(x)$ is the piecewise function
\begin{equation}
f_\epsilon(x) = 
\begin{cases}
\frac{x}{\epsilon} & 0 \leq x < \epsilon,\\
2 - \frac{x}{\epsilon} & \epsilon \leq x < 2\epsilon,\\
0 & \text{otherwise}.
\end{cases}
\end{equation}

Now, note that $f_\epsilon \to 0$ in a pointwise manner, but $f_\epsilon \not \to 0$ in $C^0$. So, how much convergence do we need to ensure that the solutions $y \to 0$ as $\epsilon \to 0$? Let us consider this using the Laplace transform.

Now we consider finding a particular solution $y_p$, i.e. a solution to $y_p'' - y_p=0$ satisfying $y_p(0) = y_p'(0) = f_\epsilon$. Letting $Y_p(s) = \mathcal L y_p$ and $F_\epsilon(s) = \mathcal L f$, we see that $(s^2 - 1)Y_p = F_\epsilon.$ Therefore, we have that $Y_p = (s^2 - 1)^{-1} F_\epsilon$. So, we get that

\begin{equation}
y_p = \int\limits_0^x \sinh(x - \tau) f_\epsilon(\tau) \dtau.
\end{equation}
Therefore,
\begin{equation}
y = c_1 \cosh x + c_2 \sinh x + \int\limits_0^x \sinh(x-\tau)f_\epsilon(\tau) \dtau.
\end{equation}

Using the boundary conditions, we get that $c_1 = 0$ and
\begin{equation}
c_2 (\epsilon) = \frac{-1}{\sinh 1} \int\limits_0^1 \sinh(1-\tau)f_\epsilon(\tau)\dtau.
\end{equation}

Since $f_\epsilon \to 0$ in $L^1$, we see that the solutions $y\to 0$ in $C^0$. Furthermore,
\begin{equation}
y' = c_2(\epsilon)\cosh x  + \int\limits_0^x \cosh(x-\tau)f_\epsilon(\tau) \dtau.
\end{equation}
So, we see that $y \to 0$ in $C^1$ as $\epsilon \to 0$. However, note that $y \not \to 0$ in $C^2$. Note that this is to be expected from Schauder estimates since $f\not \to 0$ in $C^\alpha$ for any $0<\alpha<1$.

\end{example}

%%%%%%%%%%%%%%%%%

\begin{example}
Let us consider the related example of solving the boundary value problem

\begin{equation}
\begin{cases}
y'' - y = f_\epsilon(x) & 0 < x < 1,\\
y(0) = 0,\\
y(1) = 0,
\end{cases}
\end{equation}
where $f_\epsilon$ is the piecewise function
\begin{equation}
f(x) = \begin{cases}
\frac{x}{\epsilon^2} & 0 < x < \epsilon,\\
\frac{2}{\epsilon} - \frac{x}{\epsilon^2} & \epsilon< x< 2\epsilon,\\
0 & \text{otherwise}.
\end{cases}
\end{equation}
Note that $f \not \to 0$ in $L^1$.

Let us solve this in a piecewise manner. We see that
\begin{equation}
y = \begin{cases}
-\frac{x}{\epsilon^2} + c_1 \cosh x + c_2 \sinh x & 0<x<\epsilon,\\
\frac{x}{\epsilon^2} - \frac{2}{\epsilon} + c_3 \cosh x + c_4 \sinh x & \epsilon < x < 2\epsilon,\\
c_5 \cosh x + c_6 \sinh x & 2\epsilon < x < 1.
\end{cases}
\end{equation}

To solve for the constants $c_i$, we impose the two boundary conditions plus the four conditions from demanding that $y\in C^1$.Let
\begin{equation}
M = \begin{pmatrix}
1 & 0 & 0 & 0& 0 & 0\\
1 & 0 & -1 & 0 & 0 & 0\\
0 & 1 & 0 & -1 & 0 & 0\\
0 & 0 & 1 & 0 & -1 & 0\\
0 & 0 & 0 & 1 & 0 & -1\\
0 & 0 & 0 & 0 & \cosh 1 & \sinh 1
\end{pmatrix},
\end{equation}
and
\begin{equation}
N = 
\begin{pmatrix}
0 & 0 & 0 & 0 & 0 & 0\\
0 & 1 & 0 & -1 & 0 & 0\\
1 & 0 & -1 & 0 & 0 & 0\\
0 & 0 & 0 & 1 & 0 & -1 \\
0 & 0 & 1 & 0 & -1 & 0\\
0 & 0 & 0 & 0 & 0 & 0
\end{pmatrix}
\end{equation}
Then we have that our six conditions give that
\begin{equation}\label{pde:eq_28}
(M + \epsilon N + \mathcal O (\epsilon^2)) \vec c = \begin{pmatrix}
0\\
0\\
2/\epsilon^2\\
0\\
-1/\epsilon^2\\
0
\end{pmatrix}.
\end{equation}

Now, note that one can solve 
\begin{equation}
M \vec c_0 =  \begin{pmatrix}
0\\
0\\
2\\
0\\
-1\\
0
\end{pmatrix}
\end{equation}
rather directly (without even using row reduction) to get that
\begin{equation}
\vec c_0 = \begin{pmatrix}
0\\
1\\
0\\
-1\\
0\\
0
\end{pmatrix}.
\end{equation}

Therefore, we have that
\begin{equation}
(I + M^{-1}N \epsilon + \mathcal O(\epsilon^2))\vec c = \frac{1}{\epsilon^2}\vec c_0,
\end{equation}
and so
\begin{equation}
\vec c = \frac{1}{\epsilon^2}\vec c_0 -\frac{1}{\epsilon} M^{-1}N \vec c_0 + \mathcal O(1).
\end{equation}

Now, 
\begin{equation}
N \vec c_0 = \begin{pmatrix}
0\\
2\\
0\\
-1\\
0\\
0
\end{pmatrix}.
\end{equation}

Now we solve to get that
\begin{equation}
M^{-1} N \vec c_0 = 
\begin{pmatrix}
0\\
\cosh 1 /\sinh 1\\
-2\\
\cosh 1 / \sinh 1\\
-1 \\
\cosh 1 / \sinh 1
\end{pmatrix}
\end{equation}
So, we see that
\begin{equation}
y = \begin{cases}
-\frac{x}{\epsilon^2} + \frac{1}{\epsilon^2} \sinh x +\frac{1}{\epsilon}\frac{\cosh 1}{\sinh1} \sinh x + \mathcal O(1)& 0<x<\epsilon,\\
\frac{x}{\epsilon^2} - \frac{2}{\epsilon} - \frac{1}{\epsilon^2}\sinh x - \frac{2}{\epsilon} \cosh x +\frac{1}{\epsilon}\frac{\cosh 1}{\sinh1} \sinh x+ \mathcal O(1) & \epsilon < x < 2\epsilon,\\
-\frac{1}{\epsilon}\cosh x + \frac{1}{\epsilon}\frac{\cosh 1}{\sinh1} \sinh x + \mathcal O(1)& 2\epsilon < x < 1.
\end{cases}
\end{equation}

And we may simplify some of the order to get
\begin{equation}
y = \begin{cases}
\mathcal O(1)& 0<x<\epsilon,\\
- \frac{4}{\epsilon}  +\mathcal O(1) & \epsilon < x < 2\epsilon,\\
-\frac{1}{\epsilon}+ \mathcal O(1)& 2\epsilon < x < 1.
\end{cases}
\end{equation}

So we see that $y$ doesn't even converge to $0$ in a pointwise manner as $\epsilon \to 0$.
\end{example}